theories/CTree/Logic/EF.v
@@ -38,11 +38,10 @@ Section BasicLemmas.
       φ w.
   Proof.
     intros * Hret Hcontra.
-    inv Hcontra.
-    - now rewrite ctl_now in H.
-    - destruct H0 as (? & ? & ? & ?).
-      exfalso.
-      eapply done_not_ktrans with (t:=t); eauto.
+    inv Hcontra; auto.
+    destruct H0 as (? & ? & ? & ?).
+    exfalso.
+    eapply done_not_ktrans with (t:=t); eauto.
   Qed.
 
   Lemma ef_stuck: forall w φ,
@@ -50,7 +49,8 @@ Section BasicLemmas.
       <( {Ctree.stuck: ctree E X}, w |= φ )>.
   Proof.
     split; intros.
-    - cbn in H; rewrite unfold_stuck; dependent induction H; auto.
+    - cbn in H; rewrite unfold_stuck.
+      remember Ctree.stuck in H; cdestruct H; subst.
       + now rewrite unfold_stuck in H.
       + destruct H0 as (? & ? & ? & ?).
         now apply ktrans_stuck in H0.
@@ -79,7 +79,7 @@ Section BasicLemmas.
   Proof with eauto with ctl.
     intros * Hf.
     next in Hf ; destruct Hf.
-    - rewrite ctl_vis in H; inv H...
+    - inv H; constructor.
     - destruct H as (? & ? & ? & ?).
       now apply ktrans_not_done with t x x0.
   Qed.
@@ -90,7 +90,7 @@ Section BasicLemmas.
   Proof with eauto with ctl.
     intros * Hf.
     next in Hf ; destruct Hf.
-    - rewrite ctl_pure in H; subst...
+    - subst; constructor.
     - destruct H as (? & ? & ? & ?).
       now apply ktrans_not_done with t x x0.
   Qed.
@@ -151,11 +151,16 @@ Section BasicLemmas.
     next in H; destruct H.
     - destruct H as (? & ? & ? & ?).
       ddestruction H; now ddestruction H0.
-    - next in H; destruct H as (? & ? & ? & ?).
-      ddestruction H; observe_equ x; next in H0; destruct H0;
-        rewrite <- Eqt, H in H0;
-        destruct H0 as (? & ? & ? & ?);
-        now apply ktrans_stuck in H0.
+    - destruct H as (? & ? & ? & ?).
+      ddestruction H; observe_equ x; destruct H0.
+      + rewrite <- Eqt, H in H0.
+        destruct H0 as (? & ? & ? & ?); now apply ktrans_stuck in H0.
+      + rewrite <- Eqt, H in H1.
+        destruct H1 as (? & ? & ? & ?); now apply ktrans_stuck in H1.
+      + rewrite <- Eqt, H in H0.
+        destruct H0 as (? & ? & ? & ?); now apply ktrans_stuck in H0.
+      + rewrite <- Eqt, H in H1.
+        destruct H1 as (? & ? & ? & ?); now apply ktrans_stuck in H1.
   Qed.
 
 End BasicLemmas.
@@ -174,7 +179,7 @@ Section CtlEfBind.
     induction Haf; intros; subst.
     - (* MatchA *)
       next; left; cbn.
-      apply ctl_vis in H; inv H; now constructor.
+      inv H; now constructor.
     - (* StepA *)
       destruct H0 as (t' & w' & TR' & H0).
       destruct H1 as (t_ & w_ & TR_ & H1).
@@ -197,7 +202,7 @@ Section CtlEfBind.
     induction Haf; intros; subst.
     - (* MatchA *)
       next; left; cbn.
-      apply ctl_pure in H; inv H; now constructor.
+      now apply ctl_pure. 
     - (* StepA *)
       destruct H0 as (t' & w' & TR' & H0).
       destruct H1 as (t_ & w_ & TR_ & H1).
@@ -219,7 +224,7 @@ Section CtlEfBind.
   Proof.
     intros.
     revert H0 H1.
-    induction H; intros.
+    cinduction H; intros.
     - apply ex_done in H as (Hd & y & Heqy & -> & ->).
       assert (Hk: x <- t ;; k x ~  x <- Ret y ;; k x) by (__upto_bind_sbisim; auto).
       rewrite Hk, bind_ret_l.
@@ -233,282 +238,3 @@ Section CtlEfBind.
   Admitted.
 
 End CtlEfBind.
-
-Section CtlAfIter.
-  Context {E: Type} {HE: Encode E}.
-
-  (* Total correctness lemma for [iter] *)
-  (* [Ri: I -> World E -> Prop] loop invariant (left).
-     [Rr: X -> World E -> Prop] loop postcondition (right).
-     [Rv: (I * World E) -> (I * World E) -> Prop)] loop variant (left). *)
-  Lemma af_iter{X I} Ri Rr (Rv: relation (I * World E)) (i: I) w (k: I -> ctree E (I + X)):
-    (forall (i: I) w,
-        Ri i w ->
-        <( {k i}, w |= AF AX done
-                    {fun (x: I + X) w' =>
-                       match x with
-                       | inl i' => Ri i' w' /\
-                                    Rv (i', w') (i, w)
-                       | inr r' => Rr r' w'
-                       end})>) ->
-    well_founded Rv ->
-    Ri i w ->
-    <( {iter k i}, w |= AF done Rr )>.
-  Proof.      
-    intros H WfR Hi.
-    generalize dependent k.
-    revert Hi.
-    remember (i, w) as P.
-    replace i with (fst P) by now subst.
-    replace w with (snd P) by now subst.
-    clear HeqP i w.
-    Opaque entailsF.
-    induction P using (well_founded_induction WfR);
-      destruct P as (i, w); cbn in *. 
-    rename H into HindWf.
-    intros.
-    unfold iter, MonadIter_ctree.
-    rewrite unfold_iter.
-    eapply af_bind_r with
-      (R:=fun (x : I + X) (w' : World E) =>
-            match x with
-            | inl i' => Ri i' w' /\ Rv (i', w') (i, w)
-            | inr r' => Rr r' w'
-            end); auto.
-    intros [i' | r] w'.
-    - intros (Hi' & Hv) Hd.
-      apply af_guard.
-      remember (i', w') as y.
-      replace i' with (fst y) by now subst.
-      replace w' with (snd y) by now subst.      
-      apply HindWf; inv Heqy; auto.
-    - apply af_ret. 
-  Qed.
-
-  (*| Instead of a WF relation [Rv] provide a "ranking" function [f] |*)
-  Lemma af_iter_nat{X I} Ri Rr (f: I -> World E -> nat) (i: I) w (k: I -> ctree E (I + X)):
-    (forall (i: I) w,
-        Ri i w ->
-        <( {k i}, w |= AF AX done
-                    {fun (x: I + X) w' =>
-                       match x with
-                       | inl i' => Ri i' w' /\ f i' w' < f i w
-                       | inr r' => Rr r' w'
-                       end})>) ->
-    Ri i w ->
-    <( {iter k i}, w |= AF done Rr )>.
-  Proof.
-    intros.
-    eapply af_iter with Ri (ltof _ (fun '(i, w) => f i w));
-      auto.
-    apply well_founded_ltof.
-  Qed.
-
-  Lemma af_iter_nat'{X I} Rr (f: I -> World E -> nat) (i: I) w (k: I -> ctree E (I + X)):
-    (forall (i: I) w,
-        not_done w ->
-        <( {k i}, w |= AF AX done
-                    {fun (x: I + X) w' =>
-                       match x with
-                       | inl i' => not_done w' /\ f i' w' < f i w
-                       | inr r' => Rr r' w'
-                       end})>) ->
-    not_done w ->
-    <( {iter k i}, w |= AF done Rr )>.
-  Proof.
-    intros.
-    eapply af_iter_nat with
-      (Ri:=fun _ => not_done) (f:=f); intros; auto.
-  Qed.
-
-  (* Well-founded induction on length of lists *)
-  Lemma af_iter_list{A X I} Ri Rr (f: I -> World E -> list A) (i: I) w (k: I -> ctree E (I + X)):
-    (forall (i: I) w,
-        Ri i w ->
-        <( {k i}, w |= AF AX done
-                    {fun (x: I + X) w' =>
-                       match x with
-                       | inl i' => Ri i' w' /\ length (f i' w') < length (f i w)
-                       | inr r' => Rr r' w'
-                       end})>) ->
-    Ri i w ->
-    <( {iter k i}, w |= AF done Rr )>.
-  Proof.
-    intros.
-    eapply af_iter_nat with
-      Ri (fun i w => length (f i w)); auto.
-  Qed.
-
-  Lemma af_iter_list'{A X I} Rr (f: I -> World E -> list A) (i: I) w (k: I -> ctree E (I + X)):
-    (forall (i: I) w,
-        not_done w ->
-        <( {k i}, w |= AF AX done
-                    {fun (x: I + X) w' =>
-                       match x with
-                       | inl i' => not_done w' /\
-                                    length (f i' w') < length (f i w)
-                       | inr r' => Rr r' w'
-                       end})>) ->
-    not_done w ->
-    <( {iter k i}, w |= AF done Rr )>.
-  Proof.
-    intros.
-    eapply af_iter_list with
-      (Ri:=fun _ => not_done) (f:=f); intros; auto.
-  Qed.  
-End CtlAfIter.
-
-(*| Combinators for [interp_state] |*)
-Section CtlAfState.
-  Context {E F S: Type} {HE: Encode E} {HF: Encode F}
-    (h: E ~> stateT S (ctree F)).
-
-  Theorem af_bind_state_vis{X Y}: forall s w (t: ctree E Y) (k: Y -> ctree E X) φ,
-      <( {interp_state h t s}, w |= AF vis φ )> ->
-      <( {interp_state h (x <- t ;; k x) s}, w |= AF vis φ )>.
-  Proof.
-    intros.
-    rewrite interp_state_bind.
-    now apply af_bind_vis.
-  Qed.
-  
-  Theorem af_bind_state_pure{X Y}: forall s w (t: ctree E Y) (k: Y -> ctree E X),
-      <( {interp_state h t s}, w |= AF pure )> ->
-      <( {interp_state h (x <- t ;; k x) s}, w |= AF pure )>.
-  Proof.
-    intros.
-    rewrite interp_state_bind.
-    now apply af_bind_pure.
-  Qed.
-
-  Theorem af_bind_state_r{X Y}: forall s (t: ctree E Y) (k: Y -> ctree E X) w φ (R: Y * S -> World F -> Prop),
-      <( {interp_state h t s}, w |= AF AX done R )> ->
-      (forall (y: Y) (s: S) w, R (y,s) w ->
-                    not_done w ->
-                    <( {interp_state h (k y) s}, w |= AF now φ )>) ->
-      <( {interp_state h (x <- t ;; k x) s}, w |= AF now φ )>.
-  Proof.
-    intros.
-    rewrite interp_state_bind.
-    apply af_bind_r with (R:=R); auto.
-    intros [y s'] w' Hr Hd; auto.
-  Qed.
-     
-  Theorem af_iter_state{X I} s Ri (Rr: rel (X * S) (World F))  Rv (i: I) (k: I -> ctree E (I + X)) w:
-    (forall (i: I) w s,
-        Ri i w s ->
-        <( {interp_state h (k i) s}, w |= AF AX done
-          {fun '(x, s') w' =>
-             match x with
-             | inl i' => Ri i' w' s'
-                        /\ Rv (i', w', s') (i, w, s)
-             | inr r' => Rr (r',s') w'
-             end})>) ->
-    well_founded Rv ->
-    Ri i w s ->
-    <( {interp_state h (Ctree.iter k i) s}, w |= AF done Rr )>.
-  Proof.
-    intros H WfR Hi.
-    generalize dependent k.
-    revert Hi.
-    remember (i, w, s) as P.
-    replace i with (fst (fst P)) by now subst.
-    replace w with (snd (fst P)) by now subst.
-    replace s with (snd P) by now subst.
-    clear HeqP i w s.
-    Opaque entailsF.
-    induction P using (well_founded_induction WfR);
-      destruct P as ((i, w), s); cbn in *. 
-    rename H into HindWf.
-    intros.
-    rewrite interp_state_unfold_iter.
-    eapply af_bind_r with (R:=fun '(r, s0) (w0 : World F) =>
-                      match r with
-                      | inl i' => Ri i' w0 s0 /\ Rv (i', w0, s0) (i, w, s)
-                      | inr r' => Rr (r',s0) w0
-                      end); auto.
-    intros ([i' | r] & s') w'; cbn.
-    - intros (Hi' & Hv) Hd.
-      apply af_guard.
-      remember (i', w',s') as y.
-      replace i' with (fst (fst y)) by now subst.
-      replace w' with (snd (fst y)) by now subst.
-      replace s' with (snd y) by now subst.      
-      apply HindWf; inv Heqy; auto.
-    - intros; apply af_ret; auto.
-  Qed.
-    
-  (*| Instead of a WF relation [Rv] provide a "ranking" function [f] |*)
-  Lemma af_iter_state_nat{X I} (s: S) Ri (Rr: rel (X * S) (World F)) (f: I -> World F -> S -> nat) (i: I) w
-    (k: I -> ctree E (I + X)):
-    (forall (i: I) w s,
-        Ri i w s ->
-        <( {interp_state h (k i) s}, w |= AF AX done
-                    {fun '(x, s') w' =>
-                       match x with
-                       | inl i' => Ri i' w' s' /\ f i' w' s' < f i w s
-                       | inr r' => Rr (r',s') w'
-                       end})>) ->
-    Ri i w s ->
-    <( {interp_state h (Ctree.iter k i) s}, w |= AF done Rr )>.
-  Proof.
-    intros.
-    eapply af_iter_state with Ri (ltof _ (fun '(i, w, s) => f i w s)); auto.
-    apply well_founded_ltof.
-  Qed.
-
-  Lemma af_iter_state_nat'{X I} (Rr: rel (X * S) (World F)) (f: I -> S -> nat) (s: S)
-    (i: I) w (k: I -> ctree E (I + X)):
-    (forall (i: I) w s,
-        not_done w ->
-        <( {interp_state h (k i) s}, w |= AF AX done
-                    {fun '(x, s') w' =>
-                       match x with
-                       | inl i' => not_done w' /\ f i' s' < f i s
-                       | inr r' => Rr (r',s') w'
-                       end})>) ->
-    not_done w ->
-    <( {interp_state h (Ctree.iter k i) s}, w |= AF done Rr )>.
-  Proof.
-    intros.
-    eapply af_iter_state_nat with (Ri:=fun _ w _ => not_done w) (f:=fun i _ => f i); auto.
-  Qed.
-End CtlAfState.
-
-(*| Combinators for [interp_state] with [writerE] |*)
-Section CtlAfStateList.
-  Context {E F A: Type} {HE: Encode E} {HF: Encode F} (h: E ~> stateT (list A) (ctree F)).
-
-  Lemma af_iter_state_list{X I} Ri (Rr: rel (X * list A) (World F)) (l: list A) w (i: I) (k: I -> ctree E (I + X)):
-    (forall (i: I) w (l: list A),
-        Ri i w l ->
-        <( {interp_state h (k i) l}, w |= AF AX done
-                 {fun '(x, l') w' =>
-                    match x with
-                    | inl i' => Ri i' w' l' /\ length l' < length l
-                    | inr r' => Rr (r', l') w'
-                    end})>) ->
-    Ri i w l ->
-    <( {interp_state h (Ctree.iter k i) l}, w |= AF done Rr )>.
-  Proof.
-    intros.
-    apply af_iter_state_nat with (Ri:=Ri) (f:=fun _ _ l => length l); auto.
-  Qed.
-
-  Lemma af_iter_state_list'{X I} (Rr: rel (X * list A) (World F)) (l: list A) (i: I) w (k: I -> ctree E (I + X)):
-    (forall (i: I) w (l: list A),
-        not_done w ->
-        <( {interp_state h (k i) l}, w |= AF AX done
-             {fun '(x, l') w' =>
-                match (x: I + X) with
-                | inl _ => not_done w' /\ length l' < length l
-                | inr r' => Rr (r',l') w'
-                end})>) ->
-    not_done w ->
-    <( {interp_state h (Ctree.iter k i) l}, w |= AF done Rr )>.
-  Proof.
-    intros.
-    eapply af_iter_state_list with (Ri:=fun _ w _ => not_done w); auto.
-  Qed.
-
-End CtlAfStateList.  
