theories/ITree.v
@@ -1,5 +1,0 @@
-From CTree Require Export
-  ITree.Core
-  ITree.Equ
-  Events.Core
-  Utils.Utils.
